theories/prob_lang/proofmode.v
@@ -1,0 +1,550 @@
+(* atomic.v *)
+From stdpp Require Import coPset namespaces.
+From iris.bi Require Export bi updates.
+From iris.bi.lib Require Import fixpoint.
+From iris.proofmode Require Import coq_tactics proofmode reduction.
+From iris.prelude Require Import options.
+
+(* proofmode.v *)
+From iris.proofmode Require Import coq_tactics reduction spec_patterns.
+From iris.proofmode Require Export tactics.
+From iris.program_logic Require Import atomic.
+(* From iris.heap_lang Require Export tactics derived_laws. *)
+(* From iris.heap_lang Require Import notation. *)
+From iris.prelude Require Import options.
+Import uPred.
+
+From iris.proofmode Require Import coq_tactics reduction spec_patterns.
+From iris.proofmode Require Export tactics.
+(* From iris.program_logic Require Import atomic. *)
+From self.program_logic Require Import ectx_lifting (* atomic *).
+From self.prob_lang Require Import primitive_laws notation.
+From self.prob_lang Require Export tactics (* derived_laws *).
+From iris.prelude Require Import options.
+Import uPred.
+
+Lemma tac_wp_expr_eval `{!irisGS hlc Σ} Δ s E Φ e e' :
+  (∀ (e'':=e'), e = e'') →
+  envs_entails Δ (WP e' @ s; E {{ Φ }}) → envs_entails Δ (WP e @ s; E {{ Φ }}).
+Proof. by intros ->. Qed.
+(* We don't have a TWP. Skip for now. *)
+(* Lemma tac_twp_expr_eval `{!irisGS hlc Σ} Δ s E Φ e e' : *)
+(*   (∀ (e'':=e'), e = e'') → *)
+(*   envs_entails Δ (WP e' @ s; E [{ Φ }]) → envs_entails Δ (WP e @ s; E [{ Φ }]). *)
+(* Proof. by intros ->. Qed. *)
+
+Tactic Notation "wp_expr_eval" tactic3(t) :=
+  iStartProof;
+  lazymatch goal with
+  | |- envs_entails _ (wp ?s ?E ?e ?Q) =>
+    notypeclasses refine (tac_wp_expr_eval _ _ _ _ e _ _ _);
+      [let x := fresh in intros x; t; unfold x; notypeclasses refine eq_refl|]
+  (* | |- envs_entails _ (twp ?s ?E ?e ?Q) => *)
+  (*   notypeclasses refine (tac_twp_expr_eval _ _ _ _ e _ _ _); *)
+  (*     [let x := fresh in intros x; t; unfold x; notypeclasses refine eq_refl|] *)
+  | _ => fail "wp_expr_eval: not a 'wp'"
+  end.
+Ltac wp_expr_simpl := wp_expr_eval simpl.
+
+Lemma tac_wp_pure `{!prelocGS Σ} Δ Δ' s E K e1 e2 φ n Φ :
+  PureExec φ n e1 e2 →
+  φ →
+  MaybeIntoLaterNEnvs n Δ Δ' →
+  envs_entails Δ' (WP (fill K e2) @ s; E {{ Φ }}) →
+  envs_entails Δ (WP (fill K e1) @ s; E {{ Φ }}).
+Proof.
+  rewrite envs_entails_unseal=> ??? HΔ'. rewrite into_laterN_env_sound /=.
+  (* We want [pure_exec_fill] to be available to TC search locally. *)
+  pose proof @pure_exec_fill.
+  rewrite HΔ' -lifting.wp_pure_step_later //.
+  (* iIntros "Hwp !> _" => //. *)
+Qed.
+(* Lemma tac_twp_pure `{!heapGS_gen hlc Σ} Δ s E K e1 e2 φ n Φ : *)
+(*   PureExec φ n e1 e2 → *)
+(*   φ → *)
+(*   envs_entails Δ (WP (fill K e2) @ s; E [{ Φ }]) → *)
+(*   envs_entails Δ (WP (fill K e1) @ s; E [{ Φ }]). *)
+(* Proof. *)
+(*   rewrite envs_entails_unseal=> ?? ->. *)
+(*   (* We want [pure_exec_fill] to be available to TC search locally. *) *)
+(*   pose proof @pure_exec_fill. *)
+(*   rewrite -total_lifting.twp_pure_step //. *)
+(* Qed. *)
+
+Lemma tac_wp_value_nofupd `{!prelocGS Σ} Δ s E Φ v :
+  envs_entails Δ (Φ v) → envs_entails Δ (WP (Val v) @ s; E {{ Φ }}).
+Proof. rewrite envs_entails_unseal=> ->. by apply wp_value. Qed.
+(* Lemma tac_twp_value_nofupd `{!prelocGS Σ} Δ s E Φ v : *)
+(*   envs_entails Δ (Φ v) → envs_entails Δ (WP (Val v) @ s; E [{ Φ }]). *)
+(* Proof. rewrite envs_entails_unseal=> ->. by apply twp_value. Qed. *)
+
+Lemma tac_wp_value `{!prelocGS Σ} Δ s E (Φ : val → iPropI Σ) v :
+  envs_entails Δ (|={E}=> Φ v) → envs_entails Δ (WP (Val v) @ s; E {{ Φ }}).
+Proof. rewrite envs_entails_unseal=> ->. by rewrite wp_value_fupd. Qed.
+(* Lemma tac_twp_value `{!prelocGS Σ} Δ s E (Φ : val → iPropI Σ) v : *)
+(*   envs_entails Δ (|={E}=> Φ v) → envs_entails Δ (WP (Val v) @ s; E [{ Φ }]). *)
+(* Proof. rewrite envs_entails_unseal=> ->. by rewrite twp_value_fupd. Qed. *)
+
+(** Simplify the goal if it is [WP] of a value.
+  If the postcondition already allows a fupd, do not add a second one.
+  But otherwise, *do* add a fupd. This ensures that all the lemmas applied
+  here are bidirectional, so we never will make a goal unprovable. *)
+Ltac wp_value_head :=
+  lazymatch goal with
+  | |- envs_entails _ (wp ?s ?E (Val _) (λ _, fupd ?E _ _)) =>
+      eapply tac_wp_value_nofupd
+  | |- envs_entails _ (wp ?s ?E (Val _) (λ _, wp _ ?E _ _)) =>
+      eapply tac_wp_value_nofupd
+  | |- envs_entails _ (wp ?s ?E (Val _) _) =>
+      eapply tac_wp_value
+  (* | |- envs_entails _ (twp ?s ?E (Val _) (λ _, fupd ?E _ _)) => *)
+  (*     eapply tac_twp_value_nofupd *)
+  (* | |- envs_entails _ (twp ?s ?E (Val _) (λ _, twp _ ?E _ _)) => *)
+  (*     eapply tac_twp_value_nofupd *)
+  (* | |- envs_entails _ (twp ?s ?E (Val _) _) => *)
+  (*     eapply tac_twp_value *)
+  end.
+
+Ltac wp_finish :=
+  wp_expr_simpl;      (* simplify occurences of subst/fill *)
+  try wp_value_head;  (* in case we have reached a value, get rid of the WP *)
+  pm_prettify.        (* prettify ▷s caused by [MaybeIntoLaterNEnvs] and
+                         λs caused by wp_value *)
+
+Ltac solve_vals_compare_safe :=
+  (* The first branch is for when we have [vals_compare_safe] in the context.
+     The other two branches are for when either one of the branches reduces to
+     [True] or we have it in the context. *)
+  fast_done || (left; fast_done) || (right; fast_done).
+
+(** The argument [efoc] can be used to specify the construct that should be
+reduced. For example, you can write [wp_pure (EIf _ _ _)], which will search
+for an [EIf _ _ _] in the expression, and reduce it.
+
+The use of [open_constr] in this tactic is essential. It will convert all holes
+(i.e. [_]s) into evars, that later get unified when an occurences is found
+(see [unify e' efoc] in the code below). *)
+Tactic Notation "wp_pure" open_constr(efoc) :=
+  iStartProof;
+  lazymatch goal with
+  | |- envs_entails _ (wp ?s ?E ?e ?Q) =>
+    let e := eval simpl in e in
+    reshape_expr e ltac:(fun K e' =>
+      unify e' efoc;
+      eapply (tac_wp_pure _ _ _ _ K e');
+      [iSolveTC                       (* PureExec *)
+      |try solve_vals_compare_safe    (* The pure condition for PureExec --
+         handles trivial goals, including [vals_compare_safe] *)
+      |iSolveTC                       (* IntoLaters *)
+      |wp_finish                      (* new goal *)
+      ])
+    || fail "wp_pure: cannot find" efoc "in" e "or" efoc "is not a redex"
+  | |- envs_entails _ (twp ?s ?E ?e ?Q) =>
+    let e := eval simpl in e in
+    reshape_expr e ltac:(fun K e' =>
+      unify e' efoc;
+      (* eapply (tac_twp_pure _ _ _ K e'); *)
+      [iSolveTC                       (* PureExec *)
+      |try solve_vals_compare_safe    (* The pure condition for PureExec *)
+      |wp_finish                      (* new goal *)
+      ])
+    || fail "wp_pure: cannot find" efoc "in" e "or" efoc "is not a redex"
+  | _ => fail "wp_pure: not a 'wp'"
+  end.
+Tactic Notation "wp_pure" :=
+  wp_pure _.
+
+Tactic Notation "wp_pure" open_constr(efoc) "credit:" constr(H) :=
+  iStartProof;
+  let Htmp := iFresh in
+  let finish _ :=
+    pm_reduce;
+    (iDestructHyp Htmp as H || fail 2 "wp_pure:" H "is not fresh");
+    wp_finish
+    in
+  lazymatch goal with
+  | |- envs_entails _ (wp ?s ?E ?e ?Q) =>
+    let e := eval simpl in e in
+    reshape_expr e ltac:(fun K e' =>
+      unify e' efoc;
+      (* eapply (tac_wp_pure_credit _ _ _ _ Htmp K e'); *)
+      [iSolveTC                       (* PureExec *)
+      |try solve_vals_compare_safe    (* The pure condition for PureExec --
+         handles trivial goals, including [vals_compare_safe] *)
+      |iSolveTC                       (* IntoLaters *)
+      |finish ()                      (* new goal *)
+      ])
+    || fail "wp_pure: cannot find" efoc "in" e "or" efoc "is not a redex"
+  | |- envs_entails _ (twp ?s ?E ?e ?Q) =>
+    fail "wp_pure: credit generation is not supported for a TWP"
+  | _ => fail "wp_pure: not a 'wp'"
+  end.
+Tactic Notation "wp_pure" "credit:" constr(H) :=
+  wp_pure _ credit: H.
+
+(* TODO: do this in one go, without [repeat]. *)
+Ltac wp_pures :=
+  iStartProof;
+  first [ (* The `;[]` makes sure that no side-condition magically spawns. *)
+          progress repeat (wp_pure _; [])
+        | wp_finish (* In case wp_pure never ran, make sure we do the usual cleanup. *)
+        ].
+
+(** Unlike [wp_pures], the tactics [wp_rec] and [wp_lam] should also reduce
+lambdas/recs that are hidden behind a definition, i.e. they should use
+[AsRecV_recv] as a proper instance instead of a [Hint Extern].
+
+We achieve this by putting [AsRecV_recv] in the current environment so that it
+can be used as an instance by the typeclass resolution system. We then perform
+the reduction, and finally we clear this new hypothesis. *)
+Tactic Notation "wp_rec" :=
+  let H := fresh in
+  assert (H := AsRecV_recv);
+  wp_pure (App _ _);
+  clear H.
+
+Tactic Notation "wp_if" := wp_pure (If _ _ _).
+Tactic Notation "wp_if_true" := wp_pure (If (LitV (LitBool true)) _ _).
+Tactic Notation "wp_if_false" := wp_pure (If (LitV (LitBool false)) _ _).
+Tactic Notation "wp_unop" := wp_pure (UnOp _ _).
+Tactic Notation "wp_binop" := wp_pure (BinOp _ _ _).
+Tactic Notation "wp_op" := wp_unop || wp_binop.
+Tactic Notation "wp_lam" := wp_rec.
+Tactic Notation "wp_let" := wp_pure (Rec BAnon (BNamed _) _); wp_lam.
+Tactic Notation "wp_seq" := wp_pure (Rec BAnon BAnon _); wp_lam.
+Tactic Notation "wp_proj" := wp_pure (Fst _) || wp_pure (Snd _).
+Tactic Notation "wp_case" := wp_pure (Case _ _ _).
+Tactic Notation "wp_match" := wp_case; wp_pure (Rec _ _ _); wp_lam.
+Tactic Notation "wp_inj" := wp_pure (InjL _) || wp_pure (InjR _).
+Tactic Notation "wp_pair" := wp_pure (Pair _ _).
+Tactic Notation "wp_closure" := wp_pure (Rec _ _ _).
+
+Lemma tac_wp_bind `{!prelocGS Σ} K Δ s E Φ e f :
+  f = (λ e, fill K e) → (* as an eta expanded hypothesis so that we can `simpl` it *)
+  envs_entails Δ (WP e @ s; E {{ v, WP f (Val v) @ s; E {{ Φ }} }})%I →
+  envs_entails Δ (WP fill K e @ s; E {{ Φ }}).
+Proof. rewrite envs_entails_unseal=> -> ->. by apply: wp_bind. Qed.
+(* Lemma tac_twp_bind `{!heapGS_gen hlc Σ} K Δ s E Φ e f : *)
+(*   f = (λ e, fill K e) → (* as an eta expanded hypothesis so that we can `simpl` it *) *)
+(*   envs_entails Δ (WP e @ s; E [{ v, WP f (Val v) @ s; E [{ Φ }] }])%I → *)
+(*   envs_entails Δ (WP fill K e @ s; E [{ Φ }]). *)
+(* Proof. rewrite envs_entails_unseal=> -> ->. by apply: twp_bind. Qed. *)
+
+Ltac wp_bind_core K :=
+  lazymatch eval hnf in K with
+  | [] => idtac
+  | _ => eapply (tac_wp_bind K); [simpl; reflexivity|reduction.pm_prettify]
+  end.
+(* Ltac twp_bind_core K := *)
+(*   lazymatch eval hnf in K with *)
+(*   | [] => idtac *)
+(*   | _ => eapply (tac_twp_bind K); [simpl; reflexivity|reduction.pm_prettify] *)
+(*   end. *)
+
+Tactic Notation "wp_bind" open_constr(efoc) :=
+  iStartProof;
+  lazymatch goal with
+  | |- envs_entails _ (wp ?s ?E ?e ?Q) =>
+    first [ reshape_expr e ltac:(fun K e' => unify e' efoc; wp_bind_core K)
+          | fail 1 "wp_bind: cannot find" efoc "in" e ]
+  (* | |- envs_entails _ (twp ?s ?E ?e ?Q) => *)
+  (*   first [ reshape_expr e ltac:(fun K e' => unify e' efoc; twp_bind_core K) *)
+  (*         | fail 1 "wp_bind: cannot find" efoc "in" e ] *)
+  | _ => fail "wp_bind: not a 'wp'"
+  end.
+
+(** Heap tactics *)
+Section heap.
+Context `{!prelocGS Σ}.
+Implicit Types P Q : iProp Σ.
+Implicit Types Φ : val → iProp Σ.
+Implicit Types Δ : envs (uPredI (iResUR Σ)).
+Implicit Types v : val.
+Implicit Types z : Z.
+
+(* Lemma tac_wp_allocN Δ Δ' s E j K v n Φ : *)
+(*   (0 < n)%Z → *)
+(*   MaybeIntoLaterNEnvs 1 Δ Δ' → *)
+(*   (∀ l, *)
+(*     match envs_app false (Esnoc Enil j (array l (DfracOwn 1) (replicate (Z.to_nat n) v))) Δ' with *)
+(*     | Some Δ'' => *)
+(*        envs_entails Δ'' (WP fill K (Val $ LitV $ LitLoc l) @ s; E {{ Φ }}) *)
+(*     | None => False *)
+(*     end) → *)
+(*   envs_entails Δ (WP fill K (AllocN (Val $ LitV $ LitInt n) (Val v)) @ s; E {{ Φ }}). *)
+(* Proof. *)
+(*   rewrite envs_entails_unseal=> ? ? HΔ. *)
+(*   rewrite -wp_bind. eapply wand_apply; first exact: wp_allocN. *)
+(*   rewrite left_id into_laterN_env_sound; apply later_mono, forall_intro=> l. *)
+(*   specialize (HΔ l). *)
+(*   destruct (envs_app _ _ _) as [Δ''|] eqn:HΔ'; [ | contradiction ]. *)
+(*   rewrite envs_app_sound //; simpl. *)
+(*   apply wand_intro_l. by rewrite (sep_elim_l (l ↦∗ _)%I) right_id wand_elim_r. *)
+(* Qed. *)
+(* Lemma tac_twp_allocN Δ s E j K v n Φ : *)
+(*   (0 < n)%Z → *)
+(*   (∀ l, *)
+(*     match envs_app false (Esnoc Enil j (array l (DfracOwn 1) (replicate (Z.to_nat n) v))) Δ with *)
+(*     | Some Δ' => *)
+(*        envs_entails Δ' (WP fill K (Val $ LitV $ LitLoc l) @ s; E [{ Φ }]) *)
+(*     | None => False *)
+(*     end) → *)
+(*   envs_entails Δ (WP fill K (AllocN (Val $ LitV $ LitInt n) (Val v)) @ s; E [{ Φ }]). *)
+(* Proof. *)
+(*   rewrite envs_entails_unseal=> ? HΔ. *)
+(*   rewrite -twp_bind. eapply wand_apply; first exact: twp_allocN. *)
+(*   rewrite left_id. apply forall_intro=> l. *)
+(*   specialize (HΔ l). *)
+(*   destruct (envs_app _ _ _) as [Δ'|] eqn:HΔ'; [ | contradiction ]. *)
+(*   rewrite envs_app_sound //; simpl. *)
+(*   apply wand_intro_l. by rewrite (sep_elim_l (l ↦∗ _)%I) right_id wand_elim_r. *)
+(* Qed. *)
+
+Lemma tac_wp_alloc Δ Δ' s E j K v Φ :
+  MaybeIntoLaterNEnvs 1 Δ Δ' →
+  (∀ l,
+    match envs_app false (Esnoc Enil j (l ↦ v)) Δ' with
+    | Some Δ'' =>
+       envs_entails Δ'' (WP fill K (Val $ LitV l) @ s; E {{ Φ }})
+    | None => False
+    end) →
+  envs_entails Δ (WP fill K (Alloc (Val v)) @ s; E {{ Φ }}).
+Proof.
+  rewrite envs_entails_unseal=> ? HΔ.
+  rewrite -wp_bind. eapply wand_apply; first exact: wp_alloc.
+  rewrite left_id into_laterN_env_sound; apply later_mono, forall_intro=> l.
+  specialize (HΔ l).
+  destruct (envs_app _ _ _) as [Δ''|] eqn:HΔ'; [ | contradiction ].
+  rewrite envs_app_sound //; simpl.
+  apply wand_intro_l.
+  (* rewrite (sep_elim_l (l ↦ v)%I). *)
+  rewrite right_id.
+  rewrite wand_elim_r.
+  done.
+Qed.
+(* Lemma tac_twp_alloc Δ s E j K v Φ : *)
+(*   (∀ l, *)
+(*     match envs_app false (Esnoc Enil j (l ↦ v)) Δ with *)
+(*     | Some Δ' => *)
+(*        envs_entails Δ' (WP fill K (Val $ LitV $ LitLoc l) @ s; E [{ Φ }]) *)
+(*     | None => False *)
+(*     end) → *)
+(*   envs_entails Δ (WP fill K (Alloc (Val v)) @ s; E [{ Φ }]). *)
+(* Proof. *)
+(*   rewrite envs_entails_unseal=> HΔ. *)
+(*   rewrite -twp_bind. eapply wand_apply; first exact: twp_alloc. *)
+(*   rewrite left_id. apply forall_intro=> l. *)
+(*   specialize (HΔ l). *)
+(*   destruct (envs_app _ _ _) as [Δ''|] eqn:HΔ'; [ | contradiction ]. *)
+(*   rewrite envs_app_sound //; simpl. *)
+(*   apply wand_intro_l. by rewrite (sep_elim_l (l ↦ v)%I) right_id wand_elim_r. *)
+(* Qed. *)
+
+Lemma tac_wp_load Δ Δ' s E i K b l q v Φ :
+  MaybeIntoLaterNEnvs 1 Δ Δ' →
+  envs_lookup i Δ' = Some (b, l ↦{q} v)%I →
+  envs_entails Δ' (WP fill K (Val v) @ s; E {{ Φ }}) →
+  envs_entails Δ (WP fill K (Load (LitV l)) @ s; E {{ Φ }}).
+Proof.
+  rewrite envs_entails_unseal=> ?? Hi.
+  rewrite -wp_bind. eapply wand_apply; first exact: wp_load.
+  rewrite into_laterN_env_sound -later_sep envs_lookup_split //; simpl.
+  apply later_mono.
+  destruct b; simpl.
+  * iIntros "[#$ He]". iIntros "_". iApply Hi. iApply "He". iFrame "#".
+  * by apply sep_mono_r, wand_mono.
+Qed.
+(* Lemma tac_twp_load Δ s E i K b l q v Φ : *)
+(*   envs_lookup i Δ = Some (b, l ↦{q} v)%I → *)
+(*   envs_entails Δ (WP fill K (Val v) @ s; E [{ Φ }]) → *)
+(*   envs_entails Δ (WP fill K (Load (LitV l)) @ s; E [{ Φ }]). *)
+(* Proof. *)
+(*   rewrite envs_entails_unseal=> ? Hi. *)
+(*   rewrite -twp_bind. eapply wand_apply; first exact: twp_load. *)
+(*   rewrite envs_lookup_split //; simpl. *)
+(*   destruct b; simpl. *)
+(*   - iIntros "[#$ He]". iIntros "_". iApply Hi. iApply "He". iFrame "#". *)
+(*   - iIntros "[$ He]". iIntros "Hl". iApply Hi. iApply "He". iFrame "Hl". *)
+(* Qed. *)
+
+Lemma tac_wp_store Δ Δ' s E i K l v v' Φ :
+  MaybeIntoLaterNEnvs 1 Δ Δ' →
+  envs_lookup i Δ' = Some (false, l ↦ v)%I →
+  match envs_simple_replace i false (Esnoc Enil i (l ↦ v')) Δ' with
+  | Some Δ'' => envs_entails Δ'' (WP fill K (Val $ LitV LitUnit) @ s; E {{ Φ }})
+  | None => False
+  end →
+  envs_entails Δ (WP fill K (Store (LitV l) (Val v')) @ s; E {{ Φ }}).
+Proof.
+  rewrite envs_entails_unseal=> ???.
+  destruct (envs_simple_replace _ _ _) as [Δ''|] eqn:HΔ''; [ | contradiction ].
+  rewrite -wp_bind. eapply wand_apply; first by eapply wp_store.
+  rewrite into_laterN_env_sound -later_sep envs_simple_replace_sound //; simpl.
+  rewrite right_id. by apply later_mono, sep_mono_r, wand_mono.
+Qed.
+(* Lemma tac_twp_store Δ s E i K l v v' Φ : *)
+(*   envs_lookup i Δ = Some (false, l ↦ v)%I → *)
+(*   match envs_simple_replace i false (Esnoc Enil i (l ↦ v')) Δ with *)
+(*   | Some Δ' => envs_entails Δ' (WP fill K (Val $ LitV LitUnit) @ s; E [{ Φ }]) *)
+(*   | None => False *)
+(*   end → *)
+(*   envs_entails Δ (WP fill K (Store (LitV l) v') @ s; E [{ Φ }]). *)
+(* Proof. *)
+(*   rewrite envs_entails_unseal. intros. *)
+(*   destruct (envs_simple_replace _ _ _) as [Δ''|] eqn:HΔ''; [ | contradiction ]. *)
+(*   rewrite -twp_bind. eapply wand_apply; first by eapply twp_store. *)
+(*   rewrite envs_simple_replace_sound //; simpl. *)
+(*   rewrite right_id. by apply sep_mono_r, wand_mono. *)
+(* Qed. *)
+End heap.
+
+(** The tactic [wp_apply_core lem tac_suc tac_fail] evaluates [lem] to a
+hypothesis [H] that can be applied, and then runs [wp_bind_core K; tac_suc H]
+for every possible evaluation context [K].
+
+- The tactic [tac_suc] should do [iApplyHyp H] to actually apply the hypothesis,
+  but can perform other operations in addition (see [wp_apply] and [awp_apply]
+  below).
+- The tactic [tac_fail cont] is called when [tac_suc H] fails for all evaluation
+  contexts [K], and can perform further operations before invoking [cont] to
+  try again.
+
+TC resolution of [lem] premises happens *after* [tac_suc H] got executed. *)
+Ltac wp_apply_core lem tac_suc tac_fail := first
+  [iPoseProofCore lem as false (fun H =>
+     lazymatch goal with
+     | |- envs_entails _ (wp ?s ?E ?e ?Q) =>
+       reshape_expr e ltac:(fun K e' =>
+         wp_bind_core K; tac_suc H)
+     (* | |- envs_entails _ (twp ?s ?E ?e ?Q) => *)
+     (*   reshape_expr e ltac:(fun K e' => *)
+     (*     twp_bind_core K; tac_suc H) *)
+     | _ => fail 1 "wp_apply: not a 'wp'"
+     end)
+  |tac_fail ltac:(fun _ => wp_apply_core lem tac_suc tac_fail)
+  |let P := type of lem in
+   fail "wp_apply: cannot apply" lem ":" P ].
+
+Tactic Notation "wp_apply" open_constr(lem) :=
+  wp_apply_core lem ltac:(fun H => iApplyHyp H; try iNext; try wp_expr_simpl)
+                    ltac:(fun cont => fail).
+Tactic Notation "wp_smart_apply" open_constr(lem) :=
+  wp_apply_core lem ltac:(fun H => iApplyHyp H; try iNext; try wp_expr_simpl)
+                    ltac:(fun cont => wp_pure _; []; cont ()).
+
+(** Tactic tailored for atomic triples: the first, simple one just runs
+[iAuIntro] on the goal, as atomic triples always have an atomic update as their
+premise. The second one additionaly does some framing: it gets rid of [Hs] from
+the context, reducing clutter. You get them all back in the continuation of the
+atomic operation. *)
+Tactic Notation "awp_apply" open_constr(lem) :=
+  wp_apply_core lem ltac:(fun H => iApplyHyp H) ltac:(fun cont => fail);
+  last iAuIntro.
+Tactic Notation "awp_apply" open_constr(lem) "without" constr(Hs) :=
+  (* Convert "list of hypothesis" into specialization pattern. *)
+  let Hs := words Hs in
+  let Hs := eval vm_compute in (INamed <$> Hs) in
+  wp_apply_core lem
+    ltac:(fun H =>
+      iApply (wp_frame_wand with
+        [SGoal $ SpecGoal GSpatial false [] Hs false]); [iAccu|iApplyHyp H])
+    ltac:(fun cont => fail);
+  last iAuIntro.
+
+Tactic Notation "wp_alloc" ident(l) "as" constr(H) :=
+  let Htmp := iFresh in
+  let finish _ :=
+    first [intros l | fail 1 "wp_alloc:" l "not fresh"];
+    pm_reduce;
+    lazymatch goal with
+    | |- False => fail 1 "wp_alloc:" H "not fresh"
+    | _ => iDestructHyp Htmp as H; wp_finish
+    end in
+  wp_pures;
+  (** The code first tries to use allocation lemma for a single reference,
+     ie, [tac_wp_alloc] (respectively, [tac_twp_alloc]).
+     If that fails, it tries to use the lemma [tac_wp_allocN]
+     (respectively, [tac_twp_allocN]) for allocating an array.
+     Notice that we could have used the array allocation lemma also for single
+     references. However, that would produce the resource l ↦∗ [v] instead of
+     l ↦ v for single references. These are logically equivalent assertions
+     but are not equal. *)
+  lazymatch goal with
+  | |- envs_entails _ (wp ?s ?E ?e ?Q) =>
+    let process_single _ :=
+        first
+          [reshape_expr e ltac:(fun K e' => eapply (tac_wp_alloc _ _ _ _ Htmp K))
+          |fail 1 "wp_alloc: cannot find 'Alloc' in" e];
+        [iSolveTC
+        |finish ()]
+    in
+    (* let process_array _ := *)
+    (*     first *)
+    (*       [reshape_expr e ltac:(fun K e' => eapply (tac_wp_allocN _ _ _ _ Htmp K)) *)
+    (*       |fail 1 "wp_alloc: cannot find 'Alloc' in" e]; *)
+    (*     [idtac|iSolveTC *)
+    (*      |finish ()] *)
+    (* in *) (process_single ()) (* || (process_array ()) *)
+  (* | |- envs_entails _ (twp ?s ?E ?e ?Q) => *)
+  (*   let process_single _ := *)
+  (*       first *)
+  (*         [reshape_expr e ltac:(fun K e' => eapply (tac_twp_alloc _ _ _ Htmp K)) *)
+  (*         |fail 1 "wp_alloc: cannot find 'Alloc' in" e]; *)
+  (*       finish () *)
+  (*   in *)
+  (*   let process_array _ := *)
+  (*       first *)
+  (*         [reshape_expr e ltac:(fun K e' => eapply (tac_twp_allocN _ _ _ Htmp K)) *)
+  (*         |fail 1 "wp_alloc: cannot find 'Alloc' in" e]; *)
+  (*       [idtac *)
+  (*       |finish ()] *)
+  (*   in (process_single ()) || (process_array ()) *)
+  | _ => fail "wp_alloc: not a 'wp'"
+  end.
+
+Tactic Notation "wp_alloc" ident(l) :=
+  wp_alloc l as "?".
+
+Tactic Notation "wp_load" :=
+  let solve_mapsto _ :=
+    let l := match goal with |- _ = Some (_, (?l ↦{_} _)%I) => l end in
+    iAssumptionCore || fail "wp_load: cannot find" l "↦ ?" in
+  wp_pures;
+  lazymatch goal with
+  | |- envs_entails _ (wp ?s ?E ?e ?Q) =>
+    first
+      [reshape_expr e ltac:(fun K e' => eapply (tac_wp_load _ _ _ _ _ K))
+      |fail 1 "wp_load: cannot find 'Load' in" e];
+    [iSolveTC
+    |solve_mapsto ()
+    |wp_finish]
+  (* | |- envs_entails _ (twp ?s ?E ?e ?Q) => *)
+  (*   first *)
+  (*     [reshape_expr e ltac:(fun K e' => eapply (tac_twp_load _ _ _ _ K)) *)
+  (*     |fail 1 "wp_load: cannot find 'Load' in" e]; *)
+  (*   [solve_mapsto () *)
+  (*   |wp_finish] *)
+  | _ => fail "wp_load: not a 'wp'"
+  end.
+
+Tactic Notation "wp_store" :=
+  let solve_mapsto _ :=
+    let l := match goal with |- _ = Some (_, (?l ↦{_} _)%I) => l end in
+    iAssumptionCore || fail "wp_store: cannot find" l "↦ ?" in
+  wp_pures;
+  lazymatch goal with
+  | |- envs_entails _ (wp ?s ?E ?e ?Q) =>
+    first
+      [reshape_expr e ltac:(fun K e' => eapply (tac_wp_store _ _ _ _ _ K))
+      |fail 1 "wp_store: cannot find 'Store' in" e];
+    [iSolveTC
+    |solve_mapsto ()
+    |pm_reduce; first [wp_seq|wp_finish]]
+  (* | |- envs_entails _ (twp ?s ?E ?e ?Q) => *)
+  (*   first *)
+  (*     [reshape_expr e ltac:(fun K e' => eapply (tac_twp_store _ _ _ _ K)) *)
+  (*     |fail 1 "wp_store: cannot find 'Store' in" e]; *)
+  (*   [solve_mapsto () *)
+  (*   |pm_reduce; first [wp_seq|wp_finish]] *)
+  | _ => fail "wp_store: not a 'wp'"
+  end.
