theories/prob_logrel/derived.v
@@ -1,0 +1,38 @@
+(** Derived rules. *)
+From stdpp Require Import coPset namespaces.
+From iris.proofmode Require Import proofmode.
+From iris.algebra Require Import list.
+From self.program_logic Require Import ectx_lifting.
+From self.proofmode Require Import spec_tactics.
+From self.prob_lang Require Import lang spec_rules ctx_subst proofmode.
+From self.prob_logrel Require Import model rel_rules.
+
+Section rules.
+  Context `{prelocGS Σ}.
+  Implicit Types A : lrel Σ.
+  Implicit Types e : expr.
+
+  Lemma refines_wand E e1 e2 A A' :
+    (REL e1 << e2 @ E : A) -∗
+    (∀ v1 v2, A v1 v2 ={⊤}=∗ A' v1 v2) -∗
+    REL e1 << e2 @ E : A'.
+  Proof.
+    iIntros "He HAA".
+    iApply (refines_bind [] [] with "He").
+    iIntros (v v') "HA /=". iApply refines_ret.
+    by iApply "HAA".
+  Qed.
+
+  Lemma refines_arrow (v v' : val) A A' :
+    □ (∀ v1 v2 : val, □(REL of_val v1 << of_val v2 : A) -∗
+      REL App v (of_val v1) << App v' (of_val v2) : A') -∗
+    REL (of_val v) << (of_val v') : (A → A')%lrel.
+  Proof.
+    iIntros "#H".
+    iApply refines_arrow_val; eauto.
+    iModIntro. iIntros (v1 v2) "#HA".
+    iApply "H". iModIntro.
+    by iApply refines_ret.
+  Qed.
+
+End rules.
