theories/prob_logrel/rel_rules.v
@@ -1,0 +1,239 @@
+(* ReLoC -- Relational logic for fine-grained concurrency *)
+(** Core ReLoC rules *)
+From stdpp Require Import coPset namespaces.
+From iris.proofmode Require Import proofmode.
+From iris.algebra Require Import list.
+From self.program_logic Require Import ectx_lifting.
+From self.proofmode Require Import spec_tactics.
+From self.prob_lang Require Import lang spec_rules ctx_subst proofmode.
+From self.prob_logrel Require Import model.
+
+Section rules.
+  Context `{!prelocGS Σ}.
+  Implicit Types A : lrel Σ.
+  Implicit Types e : expr.
+  Implicit Types v w : val.
+
+  Local Existing Instance pure_exec_fill.
+
+  (** * Primitive rules *)
+
+  (** ([fupd_refines] is defined in [logrel_binary.v]) *)
+
+  (** ** Forward reductions on the LHS *)
+
+  Lemma refines_pure_l n
+    (K' : list ectx_item) e e' t A ϕ :
+    PureExec ϕ n e e' →
+    ϕ →
+    ▷^n (REL fill K' e' << t : A)
+    ⊢ REL fill K' e << t : A.
+  Proof.
+    intros Hpure Hϕ.
+    rewrite refines_eq /refines_def.
+    iIntros "IH" ; iIntros (j) "Hs".
+    iModIntro. wp_pures.
+    iApply fupd_wp. iApply ("IH" with "Hs").
+  Qed.
+
+  Lemma refines_masked_l E n
+    (K' : list ectx_item) e e' t A ϕ :
+    PureExec ϕ n e e' →
+    ϕ →
+    (REL fill K' e' << t @ E : A)
+    ⊢ REL fill K' e << t @ E : A.
+  Proof.
+    intros Hpure Hϕ.
+    rewrite refines_eq /refines_def.
+    iIntros "IH" ; iIntros (j) "Hs /=".
+    iMod ("IH" with "Hs") as "IH".
+    iModIntro. by wp_pures.
+  Qed.
+
+  Lemma refines_wp_l K e1 t A :
+    (WP e1 {{ v,
+        REL fill K (of_val v) << t : A }})%I -∗
+    REL fill K e1 << t : A.
+  Proof.
+    rewrite refines_eq /refines_def.
+    iIntros "He".
+    iIntros (j) "Hs /=".
+    iModIntro. iApply wp_bind.
+    iApply (wp_wand with "He").
+    iIntros (v) "Hv".
+    by iMod ("Hv" with "Hs").
+  Qed.
+
+  Lemma refines_atomic_l (E : coPset) K e1 t A
+        (Hatomic : Atomic WeaklyAtomic e1) :
+   (|={⊤,E}=> WP e1 @ E {{ v,
+     REL fill K (of_val v) << t @ E : A }})%I -∗
+   REL fill K e1 << t : A.
+  Proof.
+    rewrite refines_eq /refines_def.
+    iIntros "Hlog".
+    iIntros (j) "Hs /=". iModIntro.
+    iApply wp_bind. iApply wp_atomic; auto.
+    iMod "Hlog" as "He". iModIntro.
+    iApply (wp_wand with "He").
+    iIntros (v) "Hlog".
+    by iApply ("Hlog" with "Hs").
+  Qed.
+
+  (** ** Forward reductions on the RHS *)
+
+  Lemma refines_pure_r E K' e e' t A n
+    (Hspec : nclose specN ⊆ E) ϕ :
+    PureExec ϕ n e e' →
+    ϕ →
+    (REL t << fill K' e' @ E : A)
+    ⊢ REL t << fill K' e @ E : A.
+  Proof.
+    rewrite refines_eq /refines_def => Hpure Hϕ.
+    iIntros "Hlog". iIntros (j) "Hj /=".
+    tp_pures j ; auto.
+    iApply ("Hlog" with "Hj").
+  Qed.
+
+  Lemma refines_right_bind K' K e :
+    refines_right K' (fill K e) ≡ refines_right (K ++ K') e.
+  Proof. rewrite /refines_right /=. by rewrite fill_app. Qed.
+
+  Definition refines_right_bind' := refines_right_bind.
+
+  (* A helper lemma for proving the stateful reductions for the RHS below *)
+  Lemma refines_step_r E K' e1 e2 A :
+    (∀ k, refines_right k e2 ={E}=∗
+         ∃ v, refines_right k (of_val v) ∗ REL e1 << fill K' (of_val v) @ E : A) -∗
+    REL e1 << fill K' e2 @ E : A.
+  Proof.
+    rewrite refines_eq /refines_def /=.
+    iIntros "He".
+    iIntros (K'') "Hs /=".
+    rewrite refines_right_bind /=.
+    iMod ("He" with "Hs") as (v) "[Hs He]".
+    rewrite -refines_right_bind'.
+    iSpecialize ("He" with "Hs").
+    by iApply "He".
+  Qed.
+
+  Lemma refines_store_r E K l e e' v v' A
+    (Hmasked : nclose specN ⊆ E) :
+    IntoVal e' v' →
+    l ↦ₛ v -∗
+    (l ↦ₛ v' -∗ REL e << fill K (of_val #()) @ E : A) -∗
+    REL e << fill K (#l <- e') @ E : A.
+  Proof.
+    rewrite /IntoVal. iIntros (<-) "Hl Hlog".
+    iApply refines_step_r.
+    iIntros (k) "Hk". simpl.
+    tp_store k. iModIntro. iExists _. iFrame.
+    by iApply "Hlog".
+  Qed.
+
+  Lemma refines_alloc_r E K e v t A
+    (Hmasked : nclose specN ⊆ E) :
+    IntoVal e v →
+    (∀ l : loc, l ↦ₛ v -∗ REL t << fill K (of_val #l) @ E : A)%I
+    -∗ REL t << fill K (ref e) @ E : A.
+  Proof.
+    rewrite /IntoVal. intros <-.
+    iIntros "Hlog". simpl.
+    iApply refines_step_r ; simpl.
+    iIntros (K') "HK'".
+    tp_alloc K' as l "Hl".
+    iModIntro. iExists _. iFrame. by iApply "Hlog".
+  Qed.
+
+  Lemma refines_alloctape_r E K t A
+    (Hmasked : nclose specN ⊆ E) :
+    (∀ α : loc, α ↪ₛ [] -∗ REL t << fill K (of_val #lbl:α) @ E : A)%I
+    -∗ REL t << fill K alloc @ E : A.
+  Proof.
+    rewrite /IntoVal.
+    iIntros "Hlog".
+    iApply refines_step_r.
+    iIntros (K') "HK'".
+    tp_alloctape K' as α "Hα".
+    iModIntro. iExists _. iFrame. by iApply "Hlog".
+  Qed.
+
+  Lemma refines_load_r E K l q v t A
+    (Hmasked : nclose specN ⊆ E) :
+    l ↦ₛ{q} v -∗
+    (l ↦ₛ{q} v -∗ REL t << fill K (of_val v) @ E : A)
+    -∗ REL t << (fill K !#l) @ E : A.
+  Proof.
+    iIntros "Hl Hlog".
+    iApply refines_step_r.
+    iIntros (k) "Hk".
+    tp_load k.
+    iModIntro. iExists _. iFrame. by iApply "Hlog".
+  Qed.
+
+
+  (** This rule is useful for proving that functions refine each other *)
+  Lemma refines_arrow_val (v v' : val) A A' :
+    □(∀ v1 v2, A v1 v2 -∗
+      REL App v (of_val v1) << App v' (of_val v2) : A') -∗
+    REL (of_val v) << (of_val v') : (A → A')%lrel.
+  Proof.
+    iIntros "#H".
+    iApply refines_ret. iModIntro.
+    iModIntro. iIntros (v1 v2) "HA".
+    iSpecialize ("H" with "HA").
+    by iApply "H".
+  Qed.
+
+  (** * Some derived (symbolic execution) rules *)
+
+  (** ** Stateful reductions on the LHS *)
+
+  Lemma refines_alloc_l K E e v t A :
+    IntoVal e v →
+    (|={⊤,E}=> ▷ (∀ l : loc, l ↦ v -∗
+           REL fill K (of_val #l) << t @ E : A))%I
+    -∗ REL fill K (ref e) << t : A.
+  Proof.
+    iIntros (<-) "Hlog".
+    iApply refines_atomic_l; auto.
+    iMod "Hlog". iModIntro.
+    iApply (wp_alloc _ _ v with "[//]"). iIntros "!>" (l) "?". by iApply "Hlog".
+  Qed.
+
+  Lemma refines_alloctape_l K E t A :
+    (|={⊤,E}=> ▷ (∀ α : loc, α ↪ [] -∗
+           REL fill K (of_val #lbl:α) << t @ E : A))%I
+    -∗ REL fill K alloc << t : A.
+  Proof.
+    iIntros "Hlog".
+    iApply refines_atomic_l; auto.
+    iMod "Hlog". iModIntro.
+    iApply (wp_alloc_tape _ _ with "[//]"). iIntros "!>" (l) "?". by iApply "Hlog".
+  Qed.
+
+  Lemma refines_load_l K E l q t A :
+    (|={⊤,E}=> ∃ v',
+      ▷(l ↦{q} v') ∗
+      ▷(l ↦{q} v' -∗ (REL fill K (of_val v') << t @ E : A)))%I
+    -∗ REL fill K (! #l) << t : A.
+  Proof.
+    iIntros "Hlog".
+    iApply refines_atomic_l; auto.
+    iMod "Hlog" as (v') "[Hl Hlog]". iModIntro.
+    iApply (wp_load with "Hl"); auto.
+  Qed.
+
+  Lemma refines_store_l K E l e v' t A :
+    IntoVal e v' →
+    (|={⊤,E}=> ∃ v, ▷ l ↦ v ∗
+      ▷(l ↦ v' -∗ REL fill K (of_val #()) << t @ E : A))
+    -∗ REL fill K (#l <- e) << t : A.
+  Proof.
+    iIntros (<-) "Hlog".
+    iApply refines_atomic_l; auto.
+    iMod "Hlog" as (v) "[Hl Hlog]". iModIntro.
+    iApply (wp_store _ _ _ _ v' with "Hl"); auto.
+  Qed.
+
+End rules.
