theories/proofmode/spec_tactics.v
@@ -1,0 +1,433 @@
+(* ReLoC -- Relational logic for fine-grained concurrency *)
+(** Tactics for updating the specification program. *)
+From iris.base_logic.lib Require Import invariants.
+From iris.proofmode Require Import
+     coq_tactics ltac_tactics
+     sel_patterns environments
+     reduction.
+From self.prob_lang Require Import spec_rules tactics.
+From self.prob_logrel Require Import model.
+Set Default Proof Using "Type".
+
+(* NB: the {pure,alloc,load,store} lemmas below have quite a bit of redundancy
+   with spec_rules.v, but they're in the shape that the proofmode tactics
+   expect, so we'll keep them around. *)
+
+(* TODO: add tp_flip *)
+
+(** ** bind *)
+Lemma tac_tp_bind_gen `{prelocGS Σ} k Δ Δ' i p e e' Q :
+  envs_lookup i Δ = Some (p, refines_right k e)%I →
+  e = e' →
+  envs_simple_replace i p (Esnoc Enil i (refines_right k e')) Δ = Some Δ' →
+  (envs_entails Δ' Q) →
+  (envs_entails Δ Q).
+Proof.
+  rewrite envs_entails_unseal. intros; subst. simpl.
+  rewrite envs_simple_replace_sound // /=.
+  destruct p; rewrite /= ?right_id; by rewrite bi.wand_elim_r.
+Qed.
+
+Lemma tac_tp_bind `{prelocGS Σ} k e' Δ Δ' i p K' e Q :
+  envs_lookup i Δ = Some (p, refines_right k e)%I →
+  e = fill K' e' →
+  envs_simple_replace i p (Esnoc Enil i (refines_right k (fill K' e'))) Δ = Some Δ' →
+  (envs_entails Δ' Q) →
+  (envs_entails Δ Q).
+Proof. intros. by eapply tac_tp_bind_gen. Qed.
+
+Ltac tp_bind_helper :=
+  simpl;
+  lazymatch goal with
+  | |- fill ?K ?e = fill _ ?efoc =>
+     reshape_expr e ltac:(fun K' e' =>
+       unify e' efoc;
+       let K'' := eval cbn[app] in (K' ++ K) in
+       replace (fill K e) with (fill K'' e') by (by rewrite ?fill_app))
+  | |- ?e = fill _ ?efoc =>
+     reshape_expr e ltac:(fun K' e' =>
+       unify e' efoc;
+       replace e with (fill K' e') by (by rewrite ?fill_app))
+  end; reflexivity.
+
+Tactic Notation "tp_normalise" constr(j) :=
+  iStartProof;
+  eapply (tac_tp_bind_gen j);
+    [iAssumptionCore (* prove the lookup *)
+    | lazymatch goal with
+      | |- fill ?K ?e = _ =>
+          by rewrite /= ?fill_app /=
+      | |- ?e = _ => try fast_done
+      end
+    |reflexivity
+    |(* new goal *)].
+
+Tactic Notation "tp_bind" constr(j) open_constr(efoc) :=
+  iStartProof;
+  eapply (tac_tp_bind j efoc);
+    [iAssumptionCore (* prove the lookup *)
+    |tp_bind_helper (* do actual work *)
+    |reflexivity
+    |(* new goal *)].
+
+Lemma tac_tp_pure `{prelocGS Σ} e K' e1 k e2 Δ1 E1 i1 e' ϕ ψ Q n :
+  (* we have those premises first, because we will be trying to solve them
+     with backtracking using reashape_expr; see the accompanying Ltac.
+     the first premise decomposes the expression, the second one checks
+     that we can make a pure step *)
+  e = fill K' e1 →
+  PureExec ϕ n e1 e2 →
+  (∀ P, ElimModal ψ false false (|={E1}=> P) P Q Q) →
+  nclose specN ⊆ E1 →
+  envs_lookup i1 Δ1 = Some (false, refines_right k e)%I →
+  ψ →
+  ϕ →
+  (* we will call simpl on this goal thus re-composing the expression again *)
+  e' = fill K' e2 →
+  match envs_simple_replace i1 false (Esnoc Enil i1 (refines_right k e')) Δ1 with
+  | Some Δ2 => envs_entails Δ2 Q
+  | None => False
+  end →
+  envs_entails Δ1 Q.
+Proof.
+  rewrite envs_entails_unseal. intros -> Hpure ?? HΔ1 Hψ Hϕ -> ?.
+  destruct (envs_simple_replace _ _ _ _) as [Δ2|] eqn:HΔ2; try done.
+  rewrite (envs_simple_replace_sound Δ1 Δ2 i1) //; simpl.
+  rewrite right_id.
+  rewrite /refines_right.
+  rewrite -!fill_app.
+  rewrite step_pure //.
+  rewrite -[Q]elim_modal // /=.
+  apply bi.sep_mono_r.
+  apply bi.wand_intro_l.
+  by rewrite bi.wand_elim_r.
+Qed.
+
+Tactic Notation "tp_pure" constr(j) open_constr(ef) :=
+  iStartProof;
+  lazymatch goal with
+  | |- context[environments.Esnoc _ ?H (refines_right j (fill ?K' ?e))] =>
+    reshape_expr e ltac:(fun K e' =>
+      unify e' ef;
+      eapply (tac_tp_pure (fill K' e) (K++K') e' j);
+      [by rewrite ?fill_app | iSolveTC | ..])
+  | |- context[environments.Esnoc _ ?H (refines_right j ?e)] =>
+    reshape_expr e ltac:(fun K e' =>
+      unify e' ef;
+      eapply (tac_tp_pure e K e' j);
+      [by rewrite ?fill_app | iSolveTC | ..])
+  end;
+  [iSolveTC || fail "tp_pure: cannot eliminate modality in the goal"
+  |solve_ndisj || fail "tp_pure: cannot prove 'nclose specN ⊆ ?'"
+  (* |iAssumptionCore || fail "tp_pure: cannot find spec_ctx" (* spec_ctx *) *)
+  |iAssumptionCore || fail "tp_pure: cannot find the RHS" (* TODO fix error message *)
+  |try (exact I || reflexivity) (* ψ *)
+  |try (exact I || reflexivity) (* ϕ *)
+  |simpl; reflexivity ||  fail "tp_pure: this should not happen" (* e' = fill K' e2 *)
+  |pm_reduce (* new goal *)].
+
+
+Tactic Notation "tp_pures" constr (j) := repeat (tp_pure j _).
+Tactic Notation "tp_rec" constr(j) :=
+  let H := fresh in
+  assert (H := AsRecV_recv);
+  tp_pure j (App _ _);
+  clear H.
+Tactic Notation "tp_seq" constr(j) := tp_rec j.
+Tactic Notation "tp_let" constr(j) := tp_rec j.
+Tactic Notation "tp_lam" constr(j) := tp_rec j.
+Tactic Notation "tp_fst" constr(j) := tp_pure j (Fst (PairV _ _)).
+Tactic Notation "tp_snd" constr(j) := tp_pure j (Snd (PairV _ _)).
+Tactic Notation "tp_proj" constr(j) := tp_pure j (_ (PairV _ _)).
+Tactic Notation "tp_case_inl" constr(j) := tp_pure j (Case (InjLV _) _ _).
+Tactic Notation "tp_case_inr" constr(j) := tp_pure j (Case (InjRV _) _ _).
+Tactic Notation "tp_case" constr(j) := tp_pure j (Case _ _ _).
+Tactic Notation "tp_binop" constr(j) := tp_pure j (BinOp _ _ _).
+Tactic Notation "tp_op" constr(j) := tp_binop j.
+Tactic Notation "tp_if_true" constr(j) := tp_pure j (If #true _ _).
+Tactic Notation "tp_if_false" constr(j) := tp_pure j (If #false _ _).
+Tactic Notation "tp_if" constr(j) := tp_pure j (If _ _ _).
+Tactic Notation "tp_pair" constr(j) := tp_pure j (Pair _ _).
+Tactic Notation "tp_closure" constr(j) := tp_pure j (Rec _ _ _).
+
+Lemma tac_tp_store `{prelocGS Σ} k Δ1 Δ2 E1 i1 i2 K' e (l : loc) e' e2 v' v Q :
+  (* TODO: here instead of True we can consider another Coq premise, like in tp_pure.
+     Same goes for the rest of those tactics *)
+  (∀ P, ElimModal True false false (|={E1}=> P) P Q Q) →
+  nclose specN ⊆ E1 →
+  envs_lookup_delete false i1 Δ1 = Some (false, refines_right k e, Δ2)%I →
+  e = fill K' (Store (# l) e') →
+  IntoVal e' v →
+  (* re-compose the expression and the evaluation context *)
+  e2 = fill K' #() →
+  envs_lookup i2 Δ2 = Some (false, l ↦ₛ v')%I →
+  match envs_simple_replace i2 false
+     (Esnoc (Esnoc Enil i1 (refines_right k e2)) i2 (l ↦ₛ v)) Δ2 with
+  | None => False
+  | Some Δ3 => envs_entails Δ3 Q
+  end →
+  envs_entails Δ1 Q.
+Proof.
+  rewrite /IntoVal.
+  rewrite envs_entails_unseal. intros ??? -> <- -> ? HQ.
+  rewrite envs_lookup_delete_sound //; simpl.
+  destruct (envs_simple_replace _ _ _ _) as [Δ3|] eqn:HΔ3; last done.
+  rewrite envs_simple_replace_sound //; simpl.
+  rewrite right_id.
+  rewrite !assoc -(assoc _ spec_ctx).
+  rewrite -fill_app step_store // fill_app.
+  rewrite -[Q]elim_modal //.
+  apply bi.sep_mono_r.
+  apply bi.wand_intro_l.
+  rewrite (comm _ _ (l ↦ₛ v)%I). simpl.
+  rewrite assoc. rewrite (comm _ spec_ctx (l ↦ₛ _)%I).
+  by rewrite bi.wand_elim_r.
+Qed.
+
+Tactic Notation "tp_store" constr(j) :=
+  iStartProof;
+  eapply (tac_tp_store j);
+  [iSolveTC || fail "tp_store: cannot eliminate modality in the goal"
+  |solve_ndisj || fail "tp_store: cannot prove 'nclose specN ⊆ ?'"
+  |iAssumptionCore || fail "tp_store: cannot find '" j " ' RHS"
+  |tp_bind_helper
+  |iSolveTC || fail "tp_store: cannot convert the argument to a value"
+  |simpl; reflexivity || fail "tp_store: this should not happen"
+  |iAssumptionCore || fail "tp_store: cannot find '? ↦ₛ ?'"
+  |pm_reduce (* new goal *)].
+
+(* *)
+(* DF: *)
+(* If [envs_lookup i1 Δ1 = Some (p, spec_ctx ρ)] and *)
+(*    [envs_lookup i2 Δ1 = Some (false, j ⤇ fill K e)], *)
+(* how can we prove that [i1 <> i2]? If we can do that then we can utilize *)
+(* the lemma [envs_lookup_envs_delete_ne]. *)
+(* *)
+
+Lemma tac_tp_load `{prelocGS Σ} k Δ1 Δ2 E1 i1 i2 K' e e2 (l : loc) v Q q :
+  (∀ P, ElimModal True false false (|={E1}=> P) P Q Q) →
+  nclose specN ⊆ E1 →
+  envs_lookup_delete false i1 Δ1 = Some (false, refines_right k e, Δ2)%I →
+  e = fill K' (Load #l) →
+  envs_lookup i2 Δ2 = Some (false, l ↦ₛ{q} v)%I →
+  e2 = fill K' (of_val v) →
+  match envs_simple_replace i2 false
+    (Esnoc (Esnoc Enil i1 (refines_right k e2)) i2 (l ↦ₛ{q} v)%I) Δ2 with
+  | Some Δ3 => envs_entails Δ3 Q
+  | None    => False
+  end →
+  envs_entails Δ1 Q.
+Proof.
+  rewrite envs_entails_unseal. intros ??? -> ? -> HQ.
+  rewrite envs_lookup_delete_sound //; simpl.
+  destruct (envs_simple_replace _ _ _ _) as [Δ3|] eqn:HΔ3; last done.
+  rewrite (envs_simple_replace_sound Δ2 Δ3 i2) //; simpl.
+  rewrite /refines_right.
+  rewrite right_id.
+  rewrite assoc. rewrite -(assoc _ spec_ctx).
+  rewrite -fill_app step_load /= // fill_app.
+  rewrite -[Q]elim_modal //.
+  apply bi.sep_mono_r.
+  apply bi.wand_intro_l.
+  rewrite (comm _ _ (l ↦ₛ{q} v)%I).
+  rewrite assoc.
+  rewrite (comm _ _ (l ↦ₛ{q} v)%I).
+  rewrite -assoc.
+  rewrite HQ. by apply bi.wand_elim_r.
+Qed.
+
+Tactic Notation "tp_load" constr(j) :=
+  iStartProof;
+  eapply (tac_tp_load j);
+  [iSolveTC || fail "tp_load: cannot eliminate modality in the goal"
+  |solve_ndisj || fail "tp_load: cannot prove 'nclose specN ⊆ ?'"
+  |iAssumptionCore || fail "tp_load: cannot find the RHS '" j "'"
+  |tp_bind_helper
+  |iAssumptionCore || fail "tp_load: cannot find '? ↦ₛ ?'"
+  |simpl; reflexivity || fail "tp_load: this should not happen"
+  |pm_reduce (* new goal *)].
+
+Lemma tac_tp_alloc `{prelocGS Σ} k Δ1 E1 i1 K' e e' v Q :
+  (∀ P, ElimModal True false false (|={E1}=> P) P Q Q) →
+  nclose specN ⊆ E1 →
+  envs_lookup i1 Δ1 = Some (false, refines_right k e)%I →
+  e = fill K' (ref e') →
+  IntoVal e' v →
+  (* TODO use match here as well *)
+  (∀ l : loc, ∃ Δ2,
+    envs_simple_replace i1 false
+       (Esnoc Enil i1 (refines_right k (fill K' #l))) Δ1 = Some Δ2 ∧
+    (envs_entails Δ2 ((l ↦ₛ v) -∗ Q)%I)) →
+  envs_entails Δ1 Q.
+Proof.
+  rewrite envs_entails_unseal. intros ??? Hfill <- HQ.
+  rewrite (envs_lookup_sound' Δ1 false i1); last by eassumption.
+  rewrite /refines_right.
+  rewrite Hfill -fill_app /=.
+  rewrite step_alloc //.
+  rewrite -[Q]elim_modal //.
+  apply bi.sep_mono_r, bi.wand_intro_l.
+  rewrite bi.sep_exist_r.
+  apply bi.exist_elim=> l.
+  destruct (HQ l) as (Δ2 & HΔ2 & HQ').
+  rewrite (envs_simple_replace_sound' _ _ i1 _ _ HΔ2) /=.
+  rewrite HQ' right_id.
+  rewrite /refines_right fill_app.
+  rewrite (comm _ _ (l ↦ₛ _)%I).
+  rewrite assoc.
+  rewrite (comm _ _ (l ↦ₛ _)%I).
+  rewrite -(assoc _ (l ↦ₛ _)%I spec_ctx _). rewrite -assoc.
+  rewrite bi.wand_elim_r.
+  by rewrite bi.wand_elim_r.
+Qed.
+
+Tactic Notation "tp_alloc" constr(j) "as" ident(l) constr(H) :=
+  let finish _ :=
+      first [ intros l | fail 1 "tp_alloc:" l "not fresh"];
+        eexists; split;
+        [ reduction.pm_reflexivity
+        | (iIntros H; tp_normalise j) || fail 1 "tp_alloc:" H "not correct intro pattern" ] in
+  iStartProof;
+  eapply (tac_tp_alloc j);
+  [iSolveTC || fail "tp_alloc: cannot eliminate modality in the goal"
+  |solve_ndisj || fail "tp_alloc: cannot prove 'nclose specN ⊆ ?'"
+  |iAssumptionCore || fail "tp_alloc: cannot find the RHS '" j "'"
+  |tp_bind_helper
+  |iSolveTC || fail "tp_alloc: expressions is not a value"
+  |finish ()
+(* new goal *)].
+
+Tactic Notation "tp_alloc" constr(j) "as" ident(j') :=
+  let H := iFresh in tp_alloc j as j' H.
+
+Lemma tac_tp_alloctape `{prelocGS Σ} k Δ1 E1 i1 K' e Q :
+  (∀ P, ElimModal True false false (|={E1}=> P) P Q Q) →
+  nclose specN ⊆ E1 →
+  envs_lookup i1 Δ1 = Some (false, refines_right k e)%I →
+  e = fill K' alloc →
+  (* TODO use match here as well *)
+  (∀ α : loc, ∃ Δ2,
+    envs_simple_replace i1 false
+       (Esnoc Enil i1 (refines_right k (fill K' #lbl:α))) Δ1 = Some Δ2 ∧
+    (envs_entails Δ2 ((α ↪ₛ []) -∗ Q)%I)) →
+  envs_entails Δ1 Q.
+Proof.
+  rewrite envs_entails_unseal. intros ??? Hfill HQ.
+  rewrite (envs_lookup_sound' Δ1 false i1); last by eassumption.
+  rewrite /refines_right.
+  rewrite Hfill -fill_app /=.
+  rewrite step_alloctape //.
+  rewrite -[Q]elim_modal //.
+  apply bi.sep_mono_r, bi.wand_intro_l.
+  rewrite bi.sep_exist_r.
+  apply bi.exist_elim=> l.
+  destruct (HQ l) as (Δ2 & HΔ2 & HQ').
+  rewrite (envs_simple_replace_sound' _ _ i1 _ _ HΔ2) /=.
+  rewrite HQ' right_id.
+  rewrite /refines_right fill_app.
+  rewrite (comm _ _ (l ↪ₛ _)%I).
+  rewrite assoc.
+  rewrite (comm _ _ (l ↪ₛ _)%I).
+  rewrite -(assoc _ (l ↪ₛ _)%I spec_ctx _). rewrite -assoc.
+  rewrite bi.wand_elim_r.
+  by rewrite bi.wand_elim_r.
+Qed.
+
+Tactic Notation "tp_alloctape" constr(j) "as" ident(l) constr(H) :=
+  let finish _ :=
+      first [ intros l | fail 1 "tp_alloctape:" l "not fresh"];
+        eexists; split;
+        [ reduction.pm_reflexivity
+        | (iIntros H; tp_normalise j) || fail 1 "tp_alloctape:" H "not correct intro pattern" ] in
+  iStartProof;
+  eapply (tac_tp_alloctape j);
+  [iSolveTC || fail "tp_alloctape: cannot eliminate modality in the goal"
+  |solve_ndisj || fail "tp_alloctape: cannot prove 'nclose specN ⊆ ?'"
+  |iAssumptionCore || fail "tp_alloctape: cannot find the RHS '" j "'"
+  |tp_bind_helper
+  |finish ()
+(* new goal *)].
+
+Tactic Notation "tp_alloctape" constr(j) "as" ident(j') :=
+  let H := iFresh in tp_alloctape j as j' H.
+
+
+(* *)
+(* (**************************) *)
+(* (* tp_apply *) *)
+
+(* Fixpoint print_sel (ss : list sel_pat) (s : string) := *)
+(*   match ss with *)
+(*   | nil => s *)
+(*   | SelPure :: ss' => (String "%" (String " " (print_sel ss' s))) *)
+(*   | SelPersistent :: ss' =>  (String "#" (print_sel ss' s)) *)
+(*   | SelSpatial :: ss' => (* no clue :( *) (print_sel ss' s) *)
+(*   | SelIdent (INamed n) :: ss' => append n (String " " (print_sel ss' s)) *)
+(*   | SelIdent (IAnon _) :: ss' => String "?" (String " " (print_sel ss' s)) *)
+(*   (* wat to do with the index? *) *)
+(*   end. *)
+
+(* Ltac print_sel ss := *)
+(*   lazymatch type of ss with *)
+(*   | list sel_pat => eval vm_compute in (print_sel ss "") *)
+(*   | string => ss *)
+(*   end. *)
+
+(* Definition appP (ss : option (list sel_pat)) (Hj Hs : string) := *)
+(*   match ss with *)
+(*   | Some ss' => cons (SelIdent Hs) (app ss' [SelIdent Hj]) *)
+(*   | None => cons (SelIdent Hs) [SelIdent Hj] *)
+(*   end. *)
+
+(* Definition add_elim_pat (pat : string) (Hj : string) := *)
+(*   match pat with *)
+(*   | EmptyString => Hj *)
+(*   | _ => append (String "[" (append Hj (String " " pat))) "]" *)
+(*   end. *)
+
+(* Tactic Notation "tp_apply" constr(j) open_constr(lem) "with" constr(Hs) "as" constr(Hr) := *)
+(*   iStartProof; *)
+(*   let rec find Γ j := *)
+(*     match Γ with *)
+(*     | Esnoc ?Γ (IAnon _) ?P => *)
+(*       find Γ j *)
+(*     | Esnoc ?Γ (INamed ?Hj) ?P => *)
+(*       lazymatch P with *)
+(*       | (j ⤇ _)%I => Hj *)
+(*       | _ => find Γ j *)
+(*       end *)
+(*     | Enil => fail 2 "tp_apply: cannot find " j " ⤇ _ " *)
+(*     | _ => fail 2 "tp_apply: unknown error in find" *)
+(*     end in *)
+(*   let rec findSpec Γp Γs := *)
+(*     match Γp with *)
+(*     | Esnoc ?Γ (IAnon _) _ => findSpec Γ Γs *)
+(*     | Esnoc ?Γ (INamed ?Hspec) ?P => *)
+(*       lazymatch P with *)
+(*       | (spec_ctx _)%I => Hspec *)
+(*       | _ => findSpec Γ Γs *)
+(*       end *)
+(*     | Enil => *)
+(*       match Γs with *)
+(*       | Enil => fail 2 "tp_apply: cannot find spec_ctx _" *)
+(*       | _ => findSpec Γs Enil *)
+(*       end *)
+(*     | _ => fail 2 "tp_apply: unknown error in findSpec" *)
+(*     end in *)
+(*   match goal with *)
+(*   | |- envs_entails (Envs ?Γp ?Γs) ?Q => *)
+(*     let Hj := (find Γs j) in *)
+(*     let Hspec := findSpec Γp Γs in *)
+(*     let pat := eval vm_compute in (appP (sel_pat.parse Hs) Hj Hspec) in *)
+(*     let pats := print_sel pat in *)
+(*     let elim_pats := eval vm_compute in (add_elim_pat Hr Hj) in *)
+(*     iMod (lem with pats) as elim_pats; first try by solve_ndisj *)
+(*   | _ => fail "tp_apply: cannot parse the context" *)
+(*   end. *)
+
+(* Tactic Notation "tp_apply" constr(j) open_constr(lem) "with" constr(Hs) := tp_apply j lem with Hs as "". *)
+
+(* Tactic Notation "tp_apply" constr(j) open_constr(lem) "as" constr(Hr) := tp_apply j lem with "" as Hr. *)
+
+(* Tactic Notation "tp_apply" constr(j) open_constr(lem) := tp_apply j lem with "" as "". *)
+(* *)
